Specify scheduling/ws_hub.

theories/scheduling/ws_hub.v
@@ -4,6 +4,8 @@
 
 From zebre Require Import
   prelude.
+From zebre.iris.base_logic Require Import
+  lib.twins.
 From zebre.language Require Import
   notations
   diaframe.
@@ -18,6 +20,12 @@ From zebre.scheduling Require Import
   ws_deques.
 From zebre Require Import
   options.
+
+Implicit Types num_round : nat.
+Implicit Types l : location.
+Implicit Types v t : val.
+Implicit Types vs : gmultiset val.
+Implicit Types γ : gname.
 
 #[local] Notation "'num_round'" := (
   in_type "t" 0
@@ -63,6 +71,7 @@ Section ws_deques.
       ws_deques.(ws_deques_push) "t".{deques} "i" "v" ;;
       ws_hub_check_waiters "t".
 
+  #[using="ws_deques"]
   Definition ws_hub_push_foreign : val :=
     λ: "t" "v",
       mpmc_queue_push "t".{foreign} "v" ;;
@@ -116,8 +125,219 @@ Section ws_deques.
       end.
 End ws_deques.
 
+Class WsHubG Σ `{zebre_G : !ZebreG Σ} := {
+  #[local] ws_hub_G_queue_G :: MpmcQueueG Σ ;
+  #[local] ws_hub_G_latch1_G :: MpscLatch1G Σ ;
+  #[local] ws_hub_G_model_G :: TwinsG Σ (leibnizO (gmultiset val)) ;
+}.
+
+Definition ws_hub_Σ := #[
+  mpmc_queue_Σ ;
+  mpsc_latch1_Σ ;
+  twins_Σ (leibnizO (gmultiset val))
+].
+#[global] Instance subG_ws_hub_Σ Σ `{zebre_G : !ZebreG Σ} :
+  subG ws_hub_Σ Σ →
+  WsHubG Σ.
+Proof.
+  solve_inG.
+Qed.
+
+Section ws_hub_G.
+  Context `{ws_hub_G : WsHubG Σ}.
+  Context (ws_deques : ws_deques Σ).
+
+  #[local] Definition ws_hub_model₁ γ vs :=
+    twins_twin1 γ (DfracOwn 1) vs.
+  #[local] Definition ws_hub_model₂ γ vs :=
+    twins_twin2 γ vs.
+
+  #[local] Definition ws_hub_inv_inner γ deques foreign waiters : iProp Σ :=
+    ∃ vs vss_deques vs_foreign latches,
+    ⌜vs = foldr (λ vs_deques vs, list_to_set_disj vs_deques ⊎ vs) ∅ vss_deques ⊎ list_to_set_disj vs_foreign⌝ ∗
+    ws_deques.(ws_deques_model) deques vss_deques ∗
+    mpmc_queue_model foreign vs_foreign ∗
+    mpmc_queue_model waiters latches ∗
+    ( [∗ list] latch ∈ latches,
+      mpsc_latch1_inv latch True
+    ) ∗
+    ws_hub_model₂ γ vs.
+  Definition ws_hub_inv t ι : iProp Σ :=
+    ∃ l γ num_round deques foreign waiters sz,
+    ⌜t = #l⌝ ∗
+    meta l nroot γ ∗
+    l.[num_round] ↦□ #num_round ∗
+    l.[deques] ↦□ deques ∗
+    l.[foreign] ↦□ foreign ∗
+    l.[waiters] ↦□ waiters ∗
+    ws_deques.(ws_deques_inv) deques ι sz ∗
+    mpmc_queue_inv foreign ι ∗
+    mpmc_queue_inv waiters ι ∗
+    inv ι (ws_hub_inv_inner γ deques foreign waiters).
+
+  #[using="ws_deques"]
+  Definition ws_hub_model t vs : iProp Σ :=
+    ∃ l γ,
+    ⌜t = #l⌝ ∗
+    meta l nroot γ ∗
+    ws_hub_model₁ γ vs.
+
+  Definition ws_hub_owner t i : iProp Σ :=
+    ∃ l γ deques,
+    ⌜t = #l⌝ ∗
+    meta l nroot γ ∗
+    l.[deques] ↦□ deques ∗
+    ws_deques.(ws_deques_owner) deques i.
+
+  #[global] Instance ws_hub_model_timeless t vs :
+    Timeless (ws_hub_model t vs).
+  Proof.
+    apply _.
+  Qed.
+  #[global] Instance ws_hub_owner_timeless t i :
+    Timeless (ws_hub_owner t i).
+  Proof.
+    apply _.
+  Qed.
+  #[global] Instance ws_hub_inv_persistent t ι :
+    Persistent (ws_hub_inv t ι).
+  Proof.
+    apply _.
+  Qed.
+
+  #[local] Lemma ws_hub_model_alloc :
+    ⊢ |==>
+      ∃ γ,
+      ws_hub_model₁ γ ∅ ∗
+      ws_hub_model₂ γ ∅.
+  Proof.
+    apply twins_alloc'.
+  Qed.
+
+  Lemma ws_hub_owner_exclusive t i :
+    ws_hub_owner t i -∗
+    ws_hub_owner t i -∗
+    False.
+  Proof.
+    iIntros "(%l & %γ & %deques & -> & _ & #Hl_deques & Howner1) (%_l & %_γ & %_deques & %Heq & _ & _Hl_deques & Howner2)". injection Heq as <-.
+    iDestruct (pointsto_agree with "Hl_deques _Hl_deques") as %<-. iClear "_Hl_deques".
+    iApply (ws_deques_owner_exclusive with "Howner1 Howner2").
+  Qed.
+
+  Lemma ws_hub_create_spec ι sz (num_round : Z) :
+    (0 ≤ sz)%Z →
+    (0 ≤ num_round)%Z →
+    {{{ True }}}
+      ws_hub_create ws_deques #sz #num_round
+    {{{ t,
+      RET t;
+      ws_hub_inv t ι ∗
+      ws_hub_model t ∅ ∗
+      [∗ list] i ∈ seq 0 (Z.to_nat sz),
+        ws_hub_owner t i
+    }}}.
+  Proof.
+    iIntros "%Hsz %Hnum_round %Φ _ HΦ".
+
+    wp_rec.
+
+    wp_smart_apply (ws_deques_create_spec with "[//]") as (deques) "(#Hdeques_inv & Hdeques_model & Hdeques_owner)"; first done.
+    wp_apply (mpmc_queue_create_spec with "[//]") as (foreign) "(#Hforeign_inv & Hforeign_model)".
+    wp_apply (mpmc_queue_create_spec with "[//]") as (waiters) "(#Hwaiters_inv & Haiters_model)".
+
+    wp_record l as "Hmeta" "(Hl_num_round & Hl_deques & Hl_foreign & Hl_waiters & _)".
+    iMod (pointsto_persist with "Hl_num_round") as "#Hl_num_round".
+    iMod (pointsto_persist with "Hl_deques") as "#Hl_deques".
+    iMod (pointsto_persist with "Hl_foreign") as "#Hl_foreign".
+    iMod (pointsto_persist with "Hl_waiters") as "#Hl_waiters".
+
+    iMod ws_hub_model_alloc as "(%γ & Hmodel₁ & Hmodel₂)".
+
+    iMod (meta_set _ _ γ with "Hmeta") as "#Hmeta"; first done.
+
+    iApply "HΦ".
+    iSplitR "Hmodel₁ Hdeques_owner".
+  Admitted.
+
+  Lemma ws_hub_push_spec t ι (i : Z) v :
+    <<<
+      ws_hub_inv t ι ∗
+      ws_hub_owner t (Z.to_nat i)
+    | ∀∀ vs,
+      ws_hub_model t vs
+    >>>
+      ws_hub_push ws_deques t #i v @ ↑ι
+    <<<
+      ws_hub_model t ({[+v+]} ⊎ vs)
+    | RET ();
+      ws_hub_owner t (Z.to_nat i)
+    >>>.
+  Proof.
+  Admitted.
+
+  Lemma ws_hub_push_foreign_spec t ι v :
+    <<<
+      ws_hub_inv t ι
+    | ∀∀ vs,
+      ws_hub_model t vs
+    >>>
+      ws_hub_push_foreign ws_deques t v @ ↑ι
+    <<<
+      ws_hub_model t ({[+v+]} ⊎ vs)
+    | RET (); True
+    >>>.
+  Proof.
+  Admitted.
+
+  Lemma ws_hub_try_pop_spec t ι (i : Z) :
+    <<<
+      ws_hub_inv t ι ∗
+      ws_hub_owner t (Z.to_nat i)
+    | ∀∀ vs,
+      ws_hub_model t vs
+    >>>
+      ws_hub_try_pop ws_deques t #i
+    <<<
+      ∃∃ o,
+      match o with
+      | None =>
+          ws_hub_model t vs
+      | Some v =>
+          ∃ v vs',
+          ⌜vs = {[+v+]} ⊎ vs'⌝ ∗
+          ws_hub_model t vs'
+      end
+    | RET o;
+      ws_hub_owner t (Z.to_nat i)
+    >>>.
+  Proof.
+  Admitted.
+
+  Lemma ws_hub_pop_spec t ι (i : Z) :
+    <<<
+      ws_hub_inv t ι ∗
+      ws_hub_owner t (Z.to_nat i)
+    | ∀∀ vs,
+      ws_hub_model t vs
+    >>>
+      ws_hub_pop ws_deques t #i
+    <<<
+      ∃∃ v vs',
+      ⌜vs = {[+v+]} ⊎ vs'⌝ ∗
+      ws_hub_model t vs'
+    | RET v;
+      ws_hub_owner t (Z.to_nat i)
+    >>>.
+  Proof.
+  Admitted.
+End ws_hub_G.
+
 #[global] Opaque ws_hub_create.
 #[global] Opaque ws_hub_push.
 #[global] Opaque ws_hub_push_foreign.
 #[global] Opaque ws_hub_try_pop.
 #[global] Opaque ws_hub_pop.
+
+#[global] Opaque ws_hub_inv.
+#[global] Opaque ws_hub_model.
+#[global] Opaque ws_hub_owner.
